tests/lean/shadow.lean
@@ -1,0 +1,9 @@
+new_frontend
+
+theorem ex1 {α} (x : α) (h : x = x) (x : α) : x = x :=
+h
+
+set_option pp.sanitizeNames false
+
+theorem ex2 {α} (x : α) (h : x = x) (x : α) : x = x :=
+h -- this error is confusing because we have disabled `pp.sanitizeNames`
